# Optellen & Aftrekken

(ook negatieve getallen; begripsvorming)





{Oefeningen}
```sums
75 - 3 =
75 - 7 =
75 - 39 =
212 - 195 =
101 - 87 =
121 - 15 - 30 =
170 - 15 + 30 =
203 - 101 - 102 =
578 -9 - 18 - 9 =
312 + 50 - 274 =
511 - 611 =
85 - 90 =
109 - 81 =
1210 - 333 =
917 - 682 =
398 + 522 =
405 - 109 - 109 =
580 - 201 - 201 - 101 =
```

{Notes; nummer verwijst naar opgave regel, geteld vanaf 1}

* 1: basic, no carry
* 2: basic, with carry a.k.a. borrow ('borrow' is the name for 'carry' when *subtracting* instead of *adding* values)
* 3: basic, multiple digits
* 6: deeper understanding possible: combine the subtracts $x-15-30 \equiv x=45$; it helps to come up with this 
     when one observes that $15=1*15$ and $30=2*15$ so in total you are subtracting $2*15+2*15=3*15=45$
* 7: deeper understanding helps, when factorization is immediately recognized: 
  $x-15+30 \equiv x-1*15+2*15 \equiv x-(1-2)*15 or x+(-1+2)*15 \equiv x+1*15 \equiv x+15$  
* 8: ditto: 101 and 102 are easily added together, thus forming $203-203$ which, surprise!, is obviously zero.
* 9: ditto, with factor 9 as a common base $=>578-1*9-2*9-1*9=578-(1+2+1)*9=578-4*9=578-36$ which is easy 
  since $8-6=2$ and $7-3=4$, i.e. both units and decades can be subtracted without having to bother with borrow anywhere.
* 11: easy to see that "we come up 100 short" (think *money*), hence the answer is a *deficit* ~ *debt*, 
  which is what is usually represented by *negative numbers*, hence we write $-100$ as the answer.
* 12: here we are "5 short", i.e. $-5$.

  Another epiphany that is lurking around the corner here is *realizing that swapping terms in a subtraction 
  flips the **sign** of the answer*: Without negative numbers, you already know that another sum, where the terms 
  have been **swapped** ($90 - 85$) has 5 as a result. Swapping the terms also results in 5 as in "we are 5 **short**", 
  i.e. **minus 5**: $90-85=5$ vs. $85-90=-5$
  
  The key insight we're gunning for is this: 
  
  + with addition you can swap terms without affecting the result: $a+b \equiv b+a$. 
    This is called [commutativity](https://en.wikipedia.org/wiki/Commutative_property) i.e. *addition is a commutative operation".
  + with subtraction, when you swap terms, you "flip" the sign (from + to - and vice versa). In other words: 
    when you swap the terms, the result is multiplied by -1 (minus one): $a-b \equiv -1 * (b-a)$, which is written shorter
    as $a-b \equiv -(b-a)$
  + a spin-off of this insight is that ${-1}*{-1}={+1}$ as that is just another way of saying "flipping the sign"
  
    (TODO) perhaps that last insight is required material *before* you can come up with the "flips the sign" insight?
    
    (TODO) ${-1}*{-1}={+1}$ turns out to be pretty tough to prove/invent --> describe in a separate page.
  

